src/PropXRel.v
@@ -1,0 +1,164 @@
+Require Import PropX PropXTac.
+Require Import Setoid Classes.Morphisms.
+
+Section machine.
+  Variable pc st : Type.
+
+  Definition PropX_imply (l r : PropX pc st) : Prop :=
+    forall cs, interp cs (Imply l r).
+  
+  Definition PropX_eq (l r : PropX pc st) : Prop :=
+    PropX_imply l r /\ PropX_imply r l.
+
+  Theorem PropX_imply_refl : Reflexive PropX_imply.
+  Proof.
+    unfold Reflexive, PropX_imply. intros.
+      eapply Imply_I. econstructor. left; auto.
+  Qed.
+
+  Theorem PropX_imply_trans : Transitive PropX_imply.
+  Proof.
+    unfold Transitive, PropX_imply. intros.
+      specialize (H cs). specialize (H0 cs).
+      eapply Imply_I. eapply Imply_E.
+      eapply valid_weaken. eassumption. compute; intros; auto.
+      eapply Imply_E. eapply valid_weaken. eassumption. compute; intros; auto.
+      propxFo.
+  Qed.
+
+  Theorem PropX_eq_refl : Reflexive PropX_eq.
+  Proof.
+    unfold Reflexive, PropX_eq. generalize PropX_imply_refl. eauto.
+  Qed.
+  
+  Theorem PropX_eq_sym : Symmetric PropX_eq.
+  Proof.
+    unfold Symmetric, PropX_eq. intuition.
+  Qed.
+
+  Theorem PropX_eq_trans : Transitive PropX_eq.
+  Proof.
+    unfold Transitive, PropX_eq. generalize PropX_imply_trans.
+      intuition;  eapply H; eauto.
+  Qed.
+
+  Add Parametric Relation : (@PropX pc st) (@PropX_imply)
+    reflexivity proved by PropX_imply_refl
+    transitivity proved by PropX_imply_trans
+  as imply_rel.
+
+  Add Parametric Relation : (@PropX pc st) (@PropX_eq)
+    reflexivity proved by PropX_eq_refl
+    symmetry proved by PropX_eq_sym
+    transitivity proved by PropX_eq_trans
+  as eq_rel.
+
+  Global Add Parametric Morphism cs : (interp cs) with
+    signature (PropX_imply ==> Basics.impl)
+  as interp_imply.
+    intros. intro. specialize (H cs). 
+    eapply Imply_E; eauto.
+  Qed.
+
+  Global Add Parametric Morphism cs : (interp cs) with
+    signature (PropX_eq ==> iff)
+  as interp_eq.
+    unfold PropX_eq.
+    intros. generalize (interp_imply cs). unfold Basics.impl. intuition;
+    eapply H0; eauto.
+  Qed.
+End machine.
+
+Require Import List.
+
+(* I'm sure this is duplication of work *)
+Section tactic.
+  Variable pcType : Type.
+  Variable stateType : Type.
+
+  Variable cs : codeSpec pcType stateType.
+
+  Lemma valid_extend : forall Ps Q R, 
+    valid cs Ps Q ->
+    valid cs (Q :: Ps) R ->
+    valid cs Ps R.
+  Proof.
+    intros.
+    eapply Imply_I in H0.
+    eapply Imply_E. eassumption.
+    eauto.
+  Qed.
+
+  Lemma valid_and_split : forall P Ps Q R, 
+    valid cs ((P /\ Q) :: Ps)%PropX R <->
+    valid cs (P :: Q :: Ps)%PropX R.
+  Proof.
+    split; intros.
+    eapply Imply_I in H. eapply Imply_E. eapply valid_weaken. eassumption.
+    firstorder.
+    eapply And_I; econstructor; firstorder.
+
+    eapply valid_extend. eapply And_E1. econstructor; firstorder.
+    eapply valid_extend. eapply And_E2. econstructor; firstorder.
+    eapply valid_weaken; eauto. firstorder.
+  Qed.
+
+  Lemma valid_perm : forall A B C,
+    valid cs (A :: B) C <->
+    valid cs (B ++ A :: nil) C.
+  Proof.
+    split; intros.
+    eapply valid_weaken; eauto. intuition.
+    eapply valid_weaken; eauto. intuition.
+    eapply incl_app; intuition. firstorder.
+  Qed.
+
+  Lemma valid_inj :  forall (A : Prop) B C,
+    (A -> valid cs B C) -> 
+    valid cs ([| A |] :: B)%PropX C.
+  Proof.
+    intros. eapply Inj_E. econstructor; firstorder. intro.
+    eapply H in H0. 
+    eapply valid_weaken; eauto. intuition.
+  Qed.
+
+  Lemma valid_ex_clear : forall T (F : T -> PropX pcType stateType) Ps R , 
+    (forall x, valid cs (F x :: Ps)%PropX R) ->
+    valid cs ((PropX.Exists F) :: Ps)%PropX R.
+  Proof.
+    intros. eapply Exists_E. econstructor. firstorder.
+    intros. eapply valid_weaken. eauto.
+    instantiate (1 := B). firstorder.
+  Qed.
+End tactic.
+
+Ltac propxIntuition :=
+  repeat (instantiate; match goal with
+                         | [ |- valid _ ((Ex x : _ , _) :: _)%PropX _ ] => 
+                           eapply valid_ex_clear; intros
+                         | [ |- valid _ ((_ /\ _) :: _)%PropX _ ] =>
+                           eapply valid_and_split
+                         | [ |- valid _ _ (_ ---> _) ] => 
+                           eapply Imply_I
+                         | [ |- valid _ ([| _ |] :: _)%PropX _ ] =>
+                           eapply valid_inj; intros
+                         | [ |- valid _ (_ :: ?X) _ ] =>
+                           match X with
+                             | context [ (_ /\ _)%PropX ] => 
+                               eapply valid_perm; simpl
+                             | context [ (Ex x : _ , _)%PropX ] => 
+                               eapply valid_perm; simpl
+                           end
+                         | [ |- valid _ _ (_ /\ _)%PropX ] =>
+                           eapply And_I
+                         | [ |- valid _ _ (Ex x : _ , _)%PropX ] =>
+                           eapply Exists_I
+                         | [ |- valid _ _ (?X _ _) ] =>
+                           match X with
+                             | @Inj _ _ => fail 1
+                             | _ =>
+                               solve [ econstructor; firstorder ]
+                           end
+                         | [ |- valid _ _ ([| _ |])%PropX ] => 
+                           eapply Inj_I
+                       end).
